-changed all Complexity-problems to be parameterised over a additional condition on the input (problems are of type 'restrictedP X').  This means that "old" problems need to be lifted using the functions defined under restrictedP in L/Complexity/Synthetic
-refactored some definitons of complecity (e.g. decInTime) to be a Record insead of a Definition with exists and /\
-renamed L_decidable_inTime to decInTime

theories/L/Complexity/NP.v
@@ -20,42 +20,41 @@ Section NP_certificate_fix.
   Definition polyBalanced R :Prop :=
     exists f, inOPoly f /\ (forall x y, R x y -> size (enc y) <= f (size (enc x))) /\ monotonic f.
 
-  Definition inTimePoly {X} `{registered X} (P : X -> Prop):=
-    exists f, L_decidable_inTime P f /\ inOPoly f /\ monotonic f.
+  Definition inTimePoly {X} `{registered X} P:=
+    exists f, decInTime P f /\ inOPoly f /\ monotonic f.
 
 
 End NP_certificate_fix.
 
-Set Warnings "-cannot-define-projection".
-Record inNP {X} `{registered X} (L : X -> Prop) : Prop :=
+Local Set Warnings "-cannot-define-projection".
+Record inNP {X} `{registered X} (P:restrictedP X) : Prop :=
   {
     (*Y : Type;
     reg__Y : registered Y;*)
     R : X -> term -> Prop; (* fixed to term for simplicity *)
-    poly__R : inTimePoly (prod_curry R);
+    poly__R : inTimePoly (fun '(x,y) => (fst (P x), R x y));
     bal__R : polyBalanced R;
-    spec__R : forall x, L x <-> exists y, R x y
+    spec__R : forall x, fst (P x) -> snd (P x) <-> exists y, R x y
   }.
 
 
-
-Lemma inNP_intro {X Y} `{_:registered X} `{registered Y} {_:decodable Y} (P : X -> Prop) (R:X -> Y -> Prop):
+Lemma inNP_intro {X Y} `{_:registered X} `{registered Y} {_:decodable Y} (P:restrictedP X) (R:X -> Y -> Prop):
   polyTimeComputable (decode Y)
-  -> inTimePoly (prod_curry R)
+  -> inTimePoly (fun '(x,y) => (fst (P x), R x y))
   -> polyBalanced R
-  ->  ( forall x, P x <-> exists y, R x y)
+  ->  ( forall x, fst (P x) -> snd(P x) <-> exists y, R x y)
   -> inNP P.
 Proof.
   intros decode__comp poly_R bal_R spec_R.
   eexists (fun x y => exists y', y = enc y' /\ R x y').
-  3:{ intro. rewrite spec_R. split;[intros (?&?)|intros (?&?&->&?)].
+  3:{ intros. rewrite spec_R. split;[intros (?&?)|intros (?&?&->&?)].
       all:repeat eexists. all:try eassumption. }
   2:{ destruct bal_R as (f&?&Hf&?). exists (fun x => f x * 11).
       all:repeat split.
       1,3:now smpl_inO.
       -intros ? ? (?&->&?). rewrite size_term_enc. rewrite Hf. 2:eassumption. cbn. reflexivity.
   }
-  { destruct poly_R as (t__f&(f&[]&?)&?&mono_t__f).
+  { destruct poly_R as (t__f&[f [] ?]&?&mono_t__f).
     destruct decode__comp as [? [] ? ? ?].
     pose (f' (x:X*term) :=
             let '(x,y):= x in
@@ -66,12 +65,12 @@ Proof.
     evar (t__f' : nat -> nat). [t__f']:intro.
     exists t__f'. repeat eapply conj.
     -exists f'. split.
-     +split. unfold f'. extract. solverec.
+     +unfold f'. extract. solverec.
       all:rewrite !size_prod. all:cbn [fst snd].
       all:hnf in polyTimeC__mono,mono_t__f.
-      *eapply decode_correct2 in H3 as <-.
-       
-       
+      *eapply decode_correct2 in H2 as <-.
+
+
        remember (size (enc a) + size (enc (enc y)) + 4) as n eqn:eqn.
        rewrite mono_t__f with (x':=n). 2:subst n;rewrite <- size_term_enc_r;lia.
        rewrite polyTimeC__mono with (x':=n). 2:lia.
@@ -80,10 +79,10 @@ Proof.
        unfold t__f'. lia.
      +unfold f'. intros []. cbn.
       destruct decode eqn:H'.
-      *etransitivity. 2:exact (H1 _). cbn.
+      *etransitivity. 2:now apply decInTime_correct. cbn iota beta.
        eapply decode_correct2 in H'. symmetry in H'.
        split;[intros (?&?&?)|intros ?].
-       --enough (x0 = y) by congruence. eapply inj_enc.  rewrite <- H', <- H3. reflexivity.
+       --cbn [snd]. enough (x0 = y) by congruence. eapply inj_enc.  rewrite <- H', <- H3. reflexivity.
        --eauto.
       *split.  2:eauto.
        intros (?&->&?). rewrite decode_correct in H'.  easy.
@@ -91,19 +90,23 @@ Proof.
     -unfold t__f'. smpl_inO.
   }
 Qed.
-  
+
 (** ** Poly Time Reduction s*)
 
 
-Definition reducesPolyMO X Y `{registered X} `{registered Y} (P : X -> Prop) (Q : Y -> Prop) :=
-  exists (f: X -> Y), polyTimeComputable f /\ forall x, (P x <-> Q (f x)).
+Record reducesPolyMO X Y `{registered X} `{registered Y} (P : restrictedP X) (Q : restrictedP Y) :Prop :=
+  {
+    reducesPolyMO_f : X -> Y;
+    reducesPolyMO_comp : polyTimeComputable reducesPolyMO_f;
+    reducesPolyMO_correct : forall x, fst (P x) -> (snd (P x) <-> snd (Q (reducesPolyMO_f x)));
+    reducesPolyMO_correctRestr : forall x, fst (P x) -> fst (Q (reducesPolyMO_f x))
+  }.
 
 Notation "P ⪯p Q" := (reducesPolyMO P Q) (at level 50).
 
-Lemma reducesPolyMO_reflexive X {regX : registered X} (P : X -> Prop) : P ⪯p P.
+Lemma reducesPolyMO_reflexive X {regX : registered X} P : P ⪯p P.
 Proof.
-  exists (fun x => x).
-  split. 2:tauto.
+  exists (fun x => x). 2,3:easy.
   exists (fun _ => 1).
   -constructor. extract. solverec.
   -smpl_inO.
@@ -111,11 +114,13 @@ Proof.
   -exists (fun x => x). repeat split. 2-3:now smpl_inO.  reflexivity.
 Qed.
 
-Lemma reducesPolyMO_transitive X Y Z {regX : registered X} {regY : registered Y} {regZ : registered Z} (P : X -> Prop) (Q : Y -> Prop) (R : Z -> Prop) :
+Lemma reducesPolyMO_transitive X Y Z {regX : registered X} {regY : registered Y} {regZ : registered Z} (P : restrictedP X) (Q : restrictedP Y) (R : restrictedP Z) :
   P ⪯p Q -> Q ⪯p R -> P ⪯p R.
 Proof.
-  intros (f&Cf&Hf) (g&Cg&Hg).
-  exists (fun x =>g (f x)). split. 2:intro;rewrite Hf,Hg;reflexivity.
+  intros [f Cf Hf Hf'] [g Cg Hg Hg'].
+  exists (fun x =>g (f x)).
+  2:now intros; rewrite Hf,Hg.
+  2:easy. 
   destruct Cf as [t__f [] ? f__mono (sizef&H__sizef&?&?)], Cg as [t__g [] ? g__mono (size__g&?&?&?)].
   exists (fun x => t__f x + t__g (sizef x) + 1).
   -split. extract. solverec.
@@ -130,26 +135,26 @@ Proof.
    +eapply monotonic_comp. all:try eassumption.
 Qed.
 
-Lemma red_inNP X Y `{regX : registered X} `{regY : registered Y} (P : X -> Prop) (Q : Y -> Prop) :
+Lemma red_inNP X Y `{regX : registered X} `{regY : registered Y} (P : restrictedP X) (Q : restrictedP Y) :
   P ⪯p Q -> inNP Q -> inNP P.
 Proof.
-  intros (f&Cf&Hf) [(*? ?*) R polyR bal specR].
+  intros [f Cf Hf] [R polyR bal specR].
 
   eexists (*_ _*) (fun x z => R (f x) z).
   -destruct Cf as [? [] ? ? (fs&H__fs&?&mono__fs)].
-   destruct polyR as (f'__t&[f' [[comp__f'] H__f']]&?&mono_f'__t).
+   destruct polyR as (f'__t&[f' [comp__f'] H__f']&?&mono_f'__t).
    eexists (fun n => polyTimeC__t n + f'__t (fs n + n) + 7). split.
    +exists (fun '(x,z)=> f' (f x,z)).
     split.
-    *split. extract. solverec.
+    *extract. solverec.
      all:rewrite !LProd.size_prod. all:cbn [fst snd].
      hnf in polyTimeC__mono,mono_f'__t,mono__fs.
      rewrite polyTimeC__mono with (x':=size (enc a) + size (enc b) + 4). 2:easy.
      erewrite mono_f'__t with (x':=_). reflexivity.
      rewrite H__fs.
      rewrite mono__fs with (x':=(size (enc a) + size (enc b) + 4)). all:Lia.nia.
-    *intros [x z]. rewrite <- H__f'.
-     cbn. reflexivity.
+    *intros [x z] ?. rewrite <- H__f'.
+     all:cbn. all:easy. 
    +split.
     all:smpl_inO.
     { eapply inOPoly_comp. all:smpl_inO. }
@@ -162,17 +167,17 @@ Proof.
     hnf in Hf__mono.
     rewrite Hf__mono. 2:eapply H__fs. reflexivity.
    +eapply monotonic_comp. all:eassumption.
-  -intros x.
-   rewrite Hf.  apply specR.
+  -intros x ?.
+   rewrite Hf. apply specR. all:easy. 
 Qed.
 
 
 (** ** NP Hardness and Completeness *)
-Definition NPhard X `{registered X} (P : X -> Prop) :=
-  forall Y `{registeredP Y} (Q : Y -> Prop),
+Definition NPhard X `{registered X} P :=
+  forall Y `{registeredP Y} Q,
     inNP Q -> Q ⪯p P.
 
-Lemma red_NPhard X Y `{registered X} `{registered Y} (P : X -> Prop) (Q: Y -> Prop)
+Lemma red_NPhard X Y `{registered X} `{registered Y} (P:restrictedP X) (Q:restrictedP Y)
   : P ⪯p Q -> NPhard P -> NPhard Q.
 Proof.
   intros R hard.
@@ -180,7 +185,7 @@ Proof.
   eapply reducesPolyMO_transitive with (1:=H'). all:eassumption.
 Qed.
 
-Definition NPcomplete X `{registered X} (P : X -> Prop) :=
+Definition NPcomplete X `{registered X} P :=
   NPhard P /\ inNP P.
 
 Hint Unfold NPcomplete.
