theories/L/Complexity/Reductions/TMGenNP/LToTMGenNP.v
@@ -9,8 +9,9 @@ From Undecidability.L Require Import TM.TMEncoding Datatypes.LFinType.
 From Undecidability.LAM  Require Import TM.HaltingProblem.
 
 
-
+(*
 Lemma polyRed_L_to_mTM : GenNPHalt ⪯p TMGenNP.
 Proof.
 
 Abort.
+*)
